Make adder used Vector type

cava/Cava/BitArithmetic.v
@@ -14,11 +14,12 @@
 (* limitations under the License.                                           *)
 (****************************************************************************)
 
-(* Bit-vector operations for Cava.
-*)
+(* Bit-vector arithmetic operations for Cava. *)
 
 From Coq Require Import Bool.Bool. 
 From Coq Require Import Lists.List.
+From Coq Require Import Vector.
+From Coq Require Import Bool.Bvector.
 Require Import Nat Arith.
 Require Import Omega.
 From Coq Require Import btauto.Btauto.
@@ -87,62 +88,62 @@ Proof. reflexivity. Qed.
 
 Example n2b_2_3 : nat_to_bits 2 3 = [true; true].
 Proof. reflexivity. Qed.
-
-(*
-Lemma twice : forall (n : nat), n + n = 2 * n.
-Proof.
-  lia.
-Qed.
-
-Lemma even_sn : forall (n : nat), even (S n) = odd (S n + 1).
-Proof.
-  intros.
-  induction n.
-  - simpl. reflexivity.
-  - unfold even.
-Abort.
-
-Lemma odd_even : forall (n : nat), odd (n + 1) = even n.
-Proof.
-  intros.
-  induction n.
-  - simpl. reflexivity.
-Abort.
-
-Lemma odd_2n_plus_1 : forall (n : nat), odd (2 * n + 1) = true.
-Proof.
-  intros.
-  induction n.
-  - simpl. reflexivity.
-Abort.
-
-Lemma first_bit: forall (a : bool) (a0 : list bool),
-               nat_to_bits (length (a :: a0)) (bits_to_nat (a :: a0)) =
-               a :: nat_to_bits (length a0) (bits_to_nat a0).
-Proof.
-  intros.
-  destruct a.
-  - simpl. rewrite plus_0_r.
-  - simpl. rewrite plus_0_r. unfold Nat.b2n. unfold odd. unfold negb.
-    destruct a.
-    + simpl. reflexivity.
-    + simpl. reflexivity.
-Abort.
-*)
-
-Lemma bits_to_from_nat : forall (a : list bool),
-                         length a > 0 ->
-                         nat_to_bits (length a) (bits_to_nat a) = a.  
-Proof.
-  intros.
-  induction a.
-  - simpl. reflexivity.
-Abort.
     
+(******************************************************************************)
+(* Functions useful for Vector operations                                     *)
+(******************************************************************************)
+
+Fixpoint bitvec_to_nat {n : nat} (bits : Bvector n) : nat :=
+  match n, bits with
+  | 0, _ => 0
+  | S n', bv => Nat.b2n (Blow n' bv) + 2 * (bitvec_to_nat (Bhigh n' bv))
+  end.
+
+Definition bv3_0 : Bvector 3 := of_list [false; false; false].
+Example bv3_0_ex : bitvec_to_nat bv3_0 = 0.
+Proof. reflexivity. Qed.
+
+Definition bv3_1 : Bvector 3 := of_list [true; false; false].
+Example bv3_1_ex : bitvec_to_nat bv3_1 = 1.
+Proof. reflexivity. Qed.
+
+Definition bv3_2 : Bvector 3 := of_list [false; true; false].
+Example bv3_2_ex : bitvec_to_nat bv3_2 = 2.
+Proof. reflexivity. Qed.
+
+
+Fixpoint nat_to_bitvec (n : nat) (v : nat) : Bvector n :=
+  match n with
+  | 0    => Bnil
+  | S n' => Bcons (testbit v 0) n' (nat_to_bitvec n' (div2 v))
+  end.
+
+Example bv3_0_exrev : nat_to_bitvec 3 0 = bv3_0.
+Proof. reflexivity. Qed.
+
+Example bv3_1_exrev : nat_to_bitvec 3 1 = bv3_1.
+Proof. reflexivity. Qed.
+
+Example bv3_2_exrev : nat_to_bitvec 3 2 = bv3_2.
+Proof. reflexivity. Qed.
+
+(* Vector version of list seq *)
+Fixpoint vec_seq (a b : nat) : Vector.t nat b :=
+  match b with
+  | 0 => Vector.nil nat
+  | S b' => Vector.cons nat a b' (vec_seq (a + 1) b')
+  end.
+
+(* Vector version of replicate *)
+Fixpoint replicate_vec {A : Type} (n : nat) (v : A) : Vector.t A n :=
+  match n with
+  | 0    => Vector.nil A
+  | S n' => Vector.cons A v n' (replicate_vec n' v)
+  end.
 
 (******************************************************************************)
 (* Functions useful for examples and tests                                    *)
 (******************************************************************************)
 
-Definition fromVec := map Nat.b2n.
-Definition toVec := map nat2bool.
+Definition fromVec := List.map Nat.b2n.
+Definition toVec := List.map nat2bool.
