cava-examples/ExamplesExtraction.v
@@ -21,6 +21,7 @@ From Coq Require Import Extraction.
 From Coq Require Import extraction.ExtrHaskellZInteger.
 From Coq Require Import extraction.ExtrHaskellString.
 From Coq Require Import ExtrHaskellBasic.
+From Coq Require Import extraction.ExtrHaskellNatInteger.
 
 Extraction Language Haskell.
 
